

K 35b

2. Find the parabola that intersects the x -axis at points $(-1, 0)$ and $(3, 0)$, and passes through point $(2, 6)$, using the following two methods.

(1) Let $y = a(x-\alpha)(x-\beta)$

[Sol] Since the parabola intersects the x -axis at $(-1, 0)$ and $(3, 0)$,

$$y = a(x+1)(x-3)$$

Since the parabola passes through $(2, 6)$,

$$6 = -3a$$

$$a = -2$$

Therefore, $y = -2(x+1)(x-3)$

$$[y = -2x^2 + 4x + 6]$$

1) $y = a(x-\alpha)(x-\beta) \leadsto$ FATORAÇÃO DA CRUZADA, INHA

$$ax^2 - (\alpha + \beta)x + \alpha\beta = 0$$

$$\beta = \alpha + \beta$$

$$\alpha = \alpha \cdot \beta$$

$$\begin{array}{rcl} x & \times & -\alpha \\ x & \times & -\beta \end{array}$$

$$\hookrightarrow [a(x-\alpha)(x-\beta)] \dots \textcircled{1}$$

SE $(-1, 0)$, $(3, 0) \rightarrow x = -1, 3$

SUBS EM $\textcircled{1}$:

$$y = a(x - (-1))(x - 3)$$

$$y = a(x+1)(x-3) \dots \textcircled{2}$$

COMO A PARABOLA PASSA POR $(2, 6)$, SUBS EM $\textcircled{2}$

$$6 = a(2+1)(2-3)$$

$$6 = a \cdot 3 \cdot (-1)$$

$$6 = -3a$$

$$a = -2$$

~~7~~

$$\boxed{-2 = a}$$

$$\therefore y = -2(x+1)(x-3) \text{ ou}$$

$$y = -2x^2 + 4x + 6$$